cp; before reorganizing files into the specs/interop directory

vale/code/arch/x64/interop/Vale.AsLowStar.Wrapper.fst
@@ -1,6 +1,11 @@
 module Vale.AsLowStar.Wrapper
 open Vale.AsLowStar.Signature
 open Vale.AsLowStar.Util
+friend X64.Interop_s
+friend X64.Memory
+friend X64.Vale.Decls
+friend X64.Vale.StateLemmas
+friend X64.Memory_Sems
 module B = LowStar.Buffer
 module BV = LowStar.BufferView
 module HS = FStar.HyperStack
@@ -13,6 +18,198 @@ module VS = X64.Vale.State
 module VSig = Vale.AsLowStar.ValeSig
 module LSig = Vale.AsLowStar.LowStarSig
 
+module TS = X64.Taint_Semantics_s
+module SL = X64.Vale.StateLemmas
+module BS = X64.Bytes_Semantics_s
+module MS = X64.Memory_Sems
+
+
+[@IS.reduce]
+let create_initial_vale_state_core
+       (acc:list ME.b8)
+       (regs:IS.registers)
+       (xmms:IS.xmms_t)
+       (taint:IS.taint_map)
+       (h0:HS.mem)
+       (stack:ME.b8{IS.mem_roots_p h0 (stack::acc)})
+  : GTot V.va_state =
+  let t_state, mem = IS.create_initial_trusted_state_core acc regs xmms taint h0 stack in
+  let open VS in
+  { ok = true;
+    regs = X64.Vale.Regs.of_fun (IS.regs_with_stack regs stack);
+    xmms = X64.Vale.Xmms.of_fun xmms;
+    flags = 0; // REVIEW
+    mem = mem;
+    memTaint = TS.(t_state.memTaint) }
+
+let lemma_create_initial_vale_state_core
+    (acc:list ME.b8)
+    (regs:IS.registers)
+    (xmms:IS.xmms_t)
+    (taint:IS.taint_map)
+    (h0:HS.mem)
+    (stack:ME.b8{IS.mem_roots_p h0 (stack::acc)})
+  : Lemma
+      (ensures (
+        let s = create_initial_vale_state_core acc regs xmms taint h0 stack in
+        VS.(ME.(s.mem.hs)) == h0
+      ))
+      [SMTPat (create_initial_vale_state_core acc regs xmms taint h0 stack)]
+  = ()
+
+let core_create_lemma
+    (acc:list ME.b8)
+    (regs:IS.registers)
+    (xmms:IS.xmms_t)
+    (taint:IS.taint_map)
+    (h0:HS.mem)
+    (stack:ME.b8{IS.mem_roots_p h0 (stack::acc)})
+  : Lemma
+      (ensures (fst (IS.create_initial_trusted_state_core acc regs xmms taint h0 stack) ==
+                SL.state_to_S (create_initial_vale_state_core acc regs xmms taint h0 stack)))
+  =
+    let s_init, mem = IS.create_initial_trusted_state_core acc regs xmms taint h0 stack in
+    let s0 = create_initial_vale_state_core acc regs xmms taint h0 stack in
+    let s1 = SL.state_to_S s0 in
+    assert (FunctionalExtensionality.feq (SL.regs' s1.TS.state) (SL.regs' s_init.TS.state));
+    assert (FunctionalExtensionality.feq (SL.xmms' s1.TS.state) (SL.xmms' s_init.TS.state))
+
+[@IS.reduce]
+let initial_vale_state_t (dom:list IS.vale_type) (acc:list ME.b8) =
+  IS.initial_state_t dom acc V.va_state
+
+[@IS.reduce]
+let create_vale_initial_state_t (dom:list IS.vale_type)
+                                (acc:list ME.b8)
+    = IS.n_dep_arrow
+          dom
+          (initial_vale_state_t dom acc)
+
+[@IS.reduce]
+let create_vale_initial_state
+      (dom:sig_arity_ok)
+    : create_vale_initial_state_t dom []
+    = IS.create_initial_state_aux
+          dom
+          IA.win
+          0
+          IA.init_regs
+          IA.init_xmms
+          []
+          IS.init_taint
+          create_initial_vale_state_core
+
+[@IS.reduce]
+let elim_down_nil (acc:list ME.b8)
+                  (down:create_vale_initial_state_t [] acc)
+    : h0:HS.mem -> stack:ME.b8{IS.mem_roots_p h0 (stack::acc)} -> GTot V.va_state =
+    down
+
+[@IS.reduce]
+let elim_down_cons (hd:IS.vale_type)
+                   (tl:list IS.vale_type)
+                   (acc:list ME.b8)
+                   (down:create_vale_initial_state_t (hd::tl) acc)
+                   (x:IS.vale_type_as_type hd)
+    : create_vale_initial_state_t tl (IS.maybe_cons_buffer hd x acc) =
+    IS.elim_dep_arrow_cons hd tl down x
+
+let rec n_dep_arrow_equiv (dom:list IS.vale_type)
+                          (acc:list ME.b8)
+                          (f:IS.create_trusted_initial_state_t dom acc)
+                          (g:create_vale_initial_state_t dom acc) =
+    match dom with
+    | [] ->
+      forall h0 (stack:ME.b8{IS.mem_roots_p h0 (stack::acc)}).
+        fst (IS.elim_down_nil acc f h0 stack) == SL.state_to_S (elim_down_nil acc g h0 stack)
+
+    | hd::tl ->
+      forall (x:IS.vale_type_as_type hd).
+        n_dep_arrow_equiv tl (IS.maybe_cons_buffer hd x acc)
+                             (IS.elim_down_cons hd tl acc f x)
+                             (elim_down_cons hd tl acc g x)
+
+let rec equiv_create_trusted_and_vale_state
+          (dom:list IS.vale_type)
+          (i:nat{i + List.length dom < IS.max_arity IA.win})
+          (regs:_)
+          (xmms:_)
+          (acc:list ME.b8)
+          (taint:_)
+    : Lemma (n_dep_arrow_equiv
+                  dom
+                  acc
+                  (IS.create_initial_state_aux
+                      dom
+                      IA.win
+                      i
+                      regs
+                      xmms
+                      acc
+                      taint
+                      IS.create_initial_trusted_state_core)
+                  (IS.create_initial_state_aux
+                      dom
+                      IA.win
+                      i
+                      regs
+                      xmms
+                      acc
+                      taint
+                      create_initial_vale_state_core))
+     = match dom with
+       | [] ->
+         FStar.Classical.forall_intro_2 (core_create_lemma acc regs xmms taint)
+       | hd::tl ->
+         let aux (x:IS.vale_type_as_type hd)
+           : Lemma (n_dep_arrow_equiv
+                      tl
+                      (IS.maybe_cons_buffer hd x acc)
+                      (IS.create_initial_state_aux
+                           tl
+                           IA.win
+                           (i + 1)
+                           (IS.update_regs x IA.win i regs)
+                           xmms
+                           (IS.maybe_cons_buffer hd x acc)
+                           (IS.update_taint_map x taint)
+                           IS.create_initial_trusted_state_core)
+                      (IS.create_initial_state_aux
+                           tl
+                           IA.win
+                           (i + 1)
+                           (IS.update_regs x IA.win i regs)
+                           xmms
+                           (IS.maybe_cons_buffer hd x acc)
+                           (IS.update_taint_map x taint)
+                           create_initial_vale_state_core))
+         =
+           equiv_create_trusted_and_vale_state
+                tl
+                (i + 1)
+                (IS.update_regs x IA.win i regs)
+                xmms
+                (IS.maybe_cons_buffer hd x acc)
+                (IS.update_taint_map x taint)
+          in
+          FStar.Classical.forall_intro aux
+
+let rec wrap_tl
+         (code:V.va_code)
+         (dom:list IS.vale_type)
+         (acc:list ME.b8)
+         (args:LSig.lowstar_args{List.length args + List.length dom < IS.max_arity IA.win})
+         (num_stack_slots:nat)
+         (fp:ME.loc)
+         (v_down:create_vale_initial_state_t dom acc)
+         (t_down:IS.create_trusted_initial_state_t dom acc{n_dep_arrow_equiv dom acc t_down v_down})
+         (pre:VSig.vale_pre_tl dom)
+         (post:VSig.vale_post_tl dom)
+         (v:VSig.vale_sig_tl fp code IA.win pre post)
+         (t_low:IS.as_lowstar_sig_tl code dom acc t_down)
+    : LSig.as_lowstar_sig_tl args num_stack_slots pre post
+    = admit()
+
 let wrap
     (code:V.va_code)
     (dom:sig_arity_ok)
@@ -21,3 +218,18 @@ let wrap
     (post:VSig.vale_post dom)
     (v:VSig.vale_sig pre post)
   : LSig.as_lowstar_sig code dom num_stack_slots pre post
+  = let is_wrapper = IS.wrap code dom in
+    equiv_create_trusted_and_vale_state dom 0 IA.init_regs IA.init_xmms [] IS.init_taint;
+    wrap_tl
+      code
+      dom
+      []
+      []
+      num_stack_slots
+      ME.loc_none
+      (create_vale_initial_state dom)
+      (IS.create_trusted_initial_state IA.win dom)
+      (pre code IA.win)
+      (post code IA.win)
+      (v code IA.win)
+      is_wrapper
